src/proofs/no_slashable_blocks/supporting_lemmas/dv_next_preserves_ind_inv/ind_inv_dv_next.dfy
@@ -46,7 +46,7 @@ module Ind_Inv_DV_Next
     import opened DV_Block_Proposer_Assumptions
     
 
-    lemma lem_ind_inv_dv_next_invs_group_1(dv: DVState, e: DVBlockEvent, dv': DVState)       
+    lemma lem_ind_inv_dv_next_invs_group_1(dv: Block_DVState, e: DVBlockEvent, dv': Block_DVState)       
     requires DV_Block_Proposer_Spec.NextEventPreCond(dv, e)
     requires DV_Block_Proposer_Spec.NextEvent(dv, e, dv')  
     requires ind_inv(dv)
@@ -59,7 +59,7 @@ module Ind_Inv_DV_Next
         lem_inv_latest_served_duty_is_a_rcvd_duty_dv_next(dv, e, dv');        
     }
 
-    lemma lem_ind_inv_dv_next_invs_group_2(dv: DVState, e: DVBlockEvent, dv': DVState)       
+    lemma lem_ind_inv_dv_next_invs_group_2(dv: Block_DVState, e: DVBlockEvent, dv': Block_DVState)       
     requires DV_Block_Proposer_Spec.NextEventPreCond(dv, e)
     requires DV_Block_Proposer_Spec.NextEvent(dv, e, dv')  
     requires ind_inv(dv)
@@ -70,7 +70,7 @@ module Ind_Inv_DV_Next
         lem_inv_available_current_proposer_duty_is_latest_proposer_duty_dv_next(dv, e, dv');        
     }
 
-    lemma lem_ind_inv_dv_next_invs_group_3(dv: DVState, e: DVBlockEvent, dv': DVState)       
+    lemma lem_ind_inv_dv_next_invs_group_3(dv: Block_DVState, e: DVBlockEvent, dv': Block_DVState)       
     requires DV_Block_Proposer_Spec.NextEventPreCond(dv, e)
     requires DV_Block_Proposer_Spec.NextEvent(dv, e, dv')  
     requires ind_inv(dv)
@@ -81,7 +81,7 @@ module Ind_Inv_DV_Next
         lem_inv_dvc_has_no_active_consensus_instances_if_latest_proposer_duty_is_none_dv_next(dv, e, dv');                        
     }
 
-    lemma lem_ind_inv_dv_next_invs_group_4(dv: DVState, e: DVBlockEvent, dv': DVState)       
+    lemma lem_ind_inv_dv_next_invs_group_4(dv: Block_DVState, e: DVBlockEvent, dv': Block_DVState)       
     requires DV_Block_Proposer_Spec.NextEventPreCond(dv, e)
     requires DV_Block_Proposer_Spec.NextEvent(dv, e, dv')  
     requires ind_inv(dv)
@@ -93,7 +93,7 @@ module Ind_Inv_DV_Next
         lem_inv_rcvd_proposer_duty_is_from_dv_seq_for_rcvd_proposer_duty_dv_next(dv, e, dv');    
     }
 
-    lemma lem_ind_inv_dv_next_invs_group_5(dv: DVState, e: DVBlockEvent, dv': DVState)       
+    lemma lem_ind_inv_dv_next_invs_group_5(dv: Block_DVState, e: DVBlockEvent, dv': Block_DVState)       
     requires DV_Block_Proposer_Spec.NextEventPreCond(dv, e)
     requires DV_Block_Proposer_Spec.NextEvent(dv, e, dv')  
     requires ind_inv(dv)
@@ -104,7 +104,7 @@ module Ind_Inv_DV_Next
         lem_inv_current_validity_predicate_for_slot_k_is_stored_in_slashing_db_hist_k_dv_next(dv, e, dv');          
     }
 
-    lemma lem_ind_inv_dv_next_invs_group_6(dv: DVState, e: DVBlockEvent, dv': DVState)       
+    lemma lem_ind_inv_dv_next_invs_group_6(dv: Block_DVState, e: DVBlockEvent, dv': Block_DVState)       
     requires DV_Block_Proposer_Spec.NextEventPreCond(dv, e)
     requires DV_Block_Proposer_Spec.NextEvent(dv, e, dv')  
     requires ind_inv(dv)
@@ -114,7 +114,7 @@ module Ind_Inv_DV_Next
         lem_inv_active_consensus_instances_are_tracked_in_slashing_db_hist_dv_next(dv, e, dv');  
     }
 
-    lemma lem_ind_inv_dv_next_invs_group_7(dv: DVState, e: DVBlockEvent, dv': DVState)       
+    lemma lem_ind_inv_dv_next_invs_group_7(dv: Block_DVState, e: DVBlockEvent, dv': Block_DVState)       
     requires DV_Block_Proposer_Spec.NextEventPreCond(dv, e)
     requires DV_Block_Proposer_Spec.NextEvent(dv, e, dv')  
     requires ind_inv(dv)
@@ -127,7 +127,7 @@ module Ind_Inv_DV_Next
         lem_inv_slots_for_sent_validity_predicates_are_stored_in_slashing_db_hist(dv, e, dv');
     }
 
-    lemma lem_ind_inv_implies_intermediate_steps_helper_1(dv: DVState)
+    lemma lem_ind_inv_implies_intermediate_steps_helper_1(dv: Block_DVState)
     requires ind_inv(dv)
     ensures inv_proposer_duty_in_next_delivery_is_higher_than_latest_served_proposer_duty(dv)
     ensures inv_proposer_duty_in_next_delivery_is_not_lower_than_rcvd_proposer_duties(dv)
@@ -136,12 +136,12 @@ module Ind_Inv_DV_Next
         lem_inv_proposer_duty_in_next_delivery_is_not_lower_than_rcvd_proposer_duties_ind_inv(dv);
     }
 
-    lemma lem_ind_inv_implies_intermediate_steps_helper_2(dv: DVState)
+    lemma lem_ind_inv_implies_intermediate_steps_helper_2(dv: Block_DVState)
     requires ind_inv(dv)  
     ensures inv_sent_vp_is_based_on_existing_slashing_db_and_rcvd_proposer_duty_and_randao_reveal(dv)
     ensures inv_active_consensus_instances_implied_the_delivery_of_proposer_duties(dv)   
     ensures inv_the_same_node_status_in_dv_and_ci(dv)    
-    ensures construct_complete_signed_block_assumptions_helper(
+    ensures construct_complete_signed_block_assumptions(
                 dv.construct_complete_signed_block,
                 dv.dv_pubkey,
                 dv.all_nodes
@@ -150,10 +150,10 @@ module Ind_Inv_DV_Next
         lem_inv_sent_vp_is_based_on_existing_slashing_db_and_rcvd_proposer_duty_and_randao_reveal_ind_inv(dv);
         lem_inv_active_consensus_instances_implied_the_delivery_of_proposer_duties_ind_inv(dv);
         lem_inv_the_same_node_status_in_dv_and_ci_ind_inv(dv);      
-        lem_construct_complete_signed_block_assumptions_helper(dv);       
+        lem_construct_complete_signed_block_assumptions(dv);       
     }
 
-    lemma lem_ind_inv_implies_intermediate_steps_helper_3(dv: DVState)
+    lemma lem_ind_inv_implies_intermediate_steps_helper_3(dv: Block_DVState)
     requires ind_inv(dv)  
     ensures inv_seq_of_proposer_duties_is_ordered(dv)
     ensures inv_active_consensus_instances_are_tracked_in_slashing_db_hist(dv)
@@ -164,7 +164,7 @@ module Ind_Inv_DV_Next
         lem_inv_rcvd_block_shares_are_from_sent_messages_inv_rcvd_block_shares_are_in_all_sent_messages(dv);
     }
 
-    lemma lem_ind_inv_implies_intermediate_steps_helper_4(dv: DVState)
+    lemma lem_ind_inv_implies_intermediate_steps_helper_4(dv: Block_DVState)
     requires ind_inv(dv)  
     ensures lem_inv_exists_honest_dvc_that_sent_block_share_for_submitted_block_new_precond(dv)    
     ensures inv_block_of_all_created_blocks_is_set_of_decided_values(dv)
@@ -175,14 +175,14 @@ module Ind_Inv_DV_Next
         lem_inv_block_of_all_created_blocks_is_set_of_decided_values_dv_next(dv);
     }
 
-    lemma lem_ind_inv_implies_intermediate_steps(dv: DVState)
+    lemma lem_ind_inv_implies_intermediate_steps(dv: Block_DVState)
     requires ind_inv(dv)
     ensures inv_proposer_duty_in_next_delivery_is_higher_than_latest_served_proposer_duty(dv)
     ensures inv_proposer_duty_in_next_delivery_is_not_lower_than_rcvd_proposer_duties(dv)
     ensures inv_sent_vp_is_based_on_existing_slashing_db_and_rcvd_proposer_duty_and_randao_reveal(dv)
     ensures inv_active_consensus_instances_implied_the_delivery_of_proposer_duties(dv)   
     ensures inv_the_same_node_status_in_dv_and_ci(dv)    
-    ensures construct_complete_signed_block_assumptions_helper(
+    ensures construct_complete_signed_block_assumptions(
                 dv.construct_complete_signed_block,
                 dv.dv_pubkey,
                 dv.all_nodes
@@ -202,7 +202,7 @@ module Ind_Inv_DV_Next
         lem_inv_block_of_all_created_blocks_is_set_of_decided_values_dv_next(dv);
     }
    
-    lemma lem_ind_inv_dv_next_invs_group_8(dv: DVState, e: DVBlockEvent, dv': DVState)       
+    lemma lem_ind_inv_dv_next_invs_group_8(dv: Block_DVState, e: DVBlockEvent, dv': Block_DVState)       
     requires DV_Block_Proposer_Spec.NextEventPreCond(dv, e)
     requires DV_Block_Proposer_Spec.NextEvent(dv, e, dv')  
     requires ind_inv(dv)
@@ -214,7 +214,7 @@ module Ind_Inv_DV_Next
         lem_inv_sent_validity_predicate_is_based_on_rcvd_proposer_duty_and_slashing_db_and_randao_reveal_dv_next(dv, e, dv');        
     }
 
-    lemma lem_ind_inv_dv_next_invs_group_9(dv: DVState, e: DVBlockEvent, dv': DVState)       
+    lemma lem_ind_inv_dv_next_invs_group_9(dv: Block_DVState, e: DVBlockEvent, dv': Block_DVState)       
     requires DV_Block_Proposer_Spec.NextEventPreCond(dv, e)
     requires DV_Block_Proposer_Spec.NextEvent(dv, e, dv')  
     requires ind_inv(dv)
@@ -226,7 +226,7 @@ module Ind_Inv_DV_Next
         lem_inv_block_shares_to_broadcast_are_sent_messages_dv_next(dv, e, dv');        
     }
 
-    lemma lem_ind_inv_dv_next_invs_group_10(dv: DVState, e: DVBlockEvent, dv': DVState)       
+    lemma lem_ind_inv_dv_next_invs_group_10(dv: Block_DVState, e: DVBlockEvent, dv': Block_DVState)       
     requires DV_Block_Proposer_Spec.NextEventPreCond(dv, e)
     requires DV_Block_Proposer_Spec.NextEvent(dv, e, dv')  
     requires ind_inv(dv)
@@ -239,7 +239,7 @@ module Ind_Inv_DV_Next
         lem_inv_exists_a_proposer_duty_in_dv_seq_of_proposer_duties_for_every_slot_in_slashing_db_hist_dv_next(dv, e, dv');
     }
     
-    lemma lem_ind_inv_dv_next_invs_group_11(dv: DVState, e: DVBlockEvent, dv': DVState)       
+    lemma lem_ind_inv_dv_next_invs_group_11(dv: Block_DVState, e: DVBlockEvent, dv': Block_DVState)       
     requires DV_Block_Proposer_Spec.NextEventPreCond(dv, e)
     requires DV_Block_Proposer_Spec.NextEvent(dv, e, dv')  
     requires ind_inv(dv)
@@ -252,7 +252,7 @@ module Ind_Inv_DV_Next
         lem_inv_unique_rcvd_proposer_duty_per_slot_dv_next(dv, e, dv');     
     }
 
-    lemma lem_ind_inv_dv_next_invs_group_12(dv: DVState, e: DVBlockEvent, dv': DVState)       
+    lemma lem_ind_inv_dv_next_invs_group_12(dv: Block_DVState, e: DVBlockEvent, dv': Block_DVState)       
     requires DV_Block_Proposer_Spec.NextEventPreCond(dv, e)
     requires DV_Block_Proposer_Spec.NextEvent(dv, e, dv')  
     requires ind_inv(dv)
@@ -265,7 +265,7 @@ module Ind_Inv_DV_Next
         lem_inv_all_validity_predicates_are_stored_in_slashing_db_hist_dv_next(dv, e, dv');
     }
 
-    lemma lem_ind_inv_dv_next_invs_group_13(dv: DVState, e: DVBlockEvent, dv': DVState)       
+    lemma lem_ind_inv_dv_next_invs_group_13(dv: Block_DVState, e: DVBlockEvent, dv': Block_DVState)       
     requires DV_Block_Proposer_Spec.NextEventPreCond(dv, e)
     requires DV_Block_Proposer_Spec.NextEvent(dv, e, dv')  
     requires ind_inv(dv)
@@ -277,7 +277,7 @@ module Ind_Inv_DV_Next
         lem_inv_exists_an_honest_dvc_as_a_witness_for_every_decided_beacon_block_dv_next(dv, e, dv');
     }
 
-    lemma lem_ind_inv_dv_next_invs_group_14(dv: DVState, e: DVBlockEvent, dv': DVState)       
+    lemma lem_ind_inv_dv_next_invs_group_14(dv: Block_DVState, e: DVBlockEvent, dv': Block_DVState)       
     requires DV_Block_Proposer_Spec.NextEventPreCond(dv, e)
     requires DV_Block_Proposer_Spec.NextEvent(dv, e, dv')  
     requires ind_inv(dv)
@@ -290,7 +290,7 @@ module Ind_Inv_DV_Next
         lem_inv_db_of_vp_contains_all_beacon_block_of_sent_block_shares_with_lower_slots_dv_next(dv, e, dv');        
     }
 
-    lemma lem_ind_inv_dv_next_invs_group_15(dv: DVState, e: DVBlockEvent, dv': DVState)       
+    lemma lem_ind_inv_dv_next_invs_group_15(dv: Block_DVState, e: DVBlockEvent, dv': Block_DVState)       
     requires DV_Block_Proposer_Spec.NextEventPreCond(dv, e)
     requires DV_Block_Proposer_Spec.NextEvent(dv, e, dv')  
     requires ind_inv(dv)
@@ -311,7 +311,7 @@ module Ind_Inv_DV_Next
         lem_inv_none_latest_slashing_db_block_implies_emply_block_slashing_db_dv_next(dv, e, dv');
     }
     
-    lemma lem_ind_inv_dv_next_ind_inv_helper_1(dv: DVState, e: DVBlockEvent, dv': DVState)       
+    lemma lem_ind_inv_dv_next_ind_inv_helper_1(dv: Block_DVState, e: DVBlockEvent, dv': Block_DVState)       
     requires DV_Block_Proposer_Spec.NextEventPreCond(dv, e)
     requires DV_Block_Proposer_Spec.NextEvent(dv, e, dv')  
     requires ind_inv(dv)
@@ -324,7 +324,7 @@ module Ind_Inv_DV_Next
         lem_ind_inv_dv_next_invs_group_3(dv, e, dv');
     }
 
-    lemma lem_ind_inv_dv_next_ind_inv_helper_2(dv: DVState, e: DVBlockEvent, dv': DVState)  
+    lemma lem_ind_inv_dv_next_ind_inv_helper_2(dv: Block_DVState, e: DVBlockEvent, dv': Block_DVState)  
     requires DV_Block_Proposer_Spec.NextEventPreCond(dv, e)
     requires DV_Block_Proposer_Spec.NextEvent(dv, e, dv')  
     requires ind_inv(dv)    
@@ -341,7 +341,7 @@ module Ind_Inv_DV_Next
         lem_ind_inv_dv_next_invs_group_8(dv, e, dv');
     }
 
-    lemma lem_ind_inv_dv_next_ind_inv_helper_3(dv: DVState, e: DVBlockEvent, dv': DVState)       
+    lemma lem_ind_inv_dv_next_ind_inv_helper_3(dv: Block_DVState, e: DVBlockEvent, dv': Block_DVState)       
     requires DV_Block_Proposer_Spec.NextEventPreCond(dv, e)
     requires DV_Block_Proposer_Spec.NextEvent(dv, e, dv')  
     requires ind_inv(dv)
@@ -354,7 +354,7 @@ module Ind_Inv_DV_Next
         lem_ind_inv_dv_next_invs_group_11(dv, e, dv');                                     
     }
 
-    lemma lem_ind_inv_dv_next_ind_inv_helper_4(dv: DVState, e: DVBlockEvent, dv': DVState)       
+    lemma lem_ind_inv_dv_next_ind_inv_helper_4(dv: Block_DVState, e: DVBlockEvent, dv': Block_DVState)       
     requires DV_Block_Proposer_Spec.NextEventPreCond(dv, e)
     requires DV_Block_Proposer_Spec.NextEvent(dv, e, dv')  
     requires ind_inv(dv)
@@ -365,7 +365,7 @@ module Ind_Inv_DV_Next
         lem_ind_inv_dv_next_invs_group_13(dv, e, dv');             
     }
 
-    lemma lem_ind_inv_dv_next_ind_inv_helper_5(dv: DVState, e: DVBlockEvent, dv': DVState)       
+    lemma lem_ind_inv_dv_next_ind_inv_helper_5(dv: Block_DVState, e: DVBlockEvent, dv': Block_DVState)       
     requires DV_Block_Proposer_Spec.NextEventPreCond(dv, e)
     requires DV_Block_Proposer_Spec.NextEvent(dv, e, dv')  
     requires ind_inv(dv)    
@@ -376,7 +376,7 @@ module Ind_Inv_DV_Next
         lem_ind_inv_dv_next_invs_group_15(dv, e, dv');                              
     }
 
-    lemma lem_ind_inv_dv_next_ind_inv_helper_a(dv: DVState, e: DVBlockEvent, dv': DVState)       
+    lemma lem_ind_inv_dv_next_ind_inv_helper_a(dv: Block_DVState, e: DVBlockEvent, dv': Block_DVState)       
     requires DV_Block_Proposer_Spec.NextEventPreCond(dv, e)
     requires DV_Block_Proposer_Spec.NextEvent(dv, e, dv')  
     requires ind_inv(dv) 
@@ -393,7 +393,7 @@ module Ind_Inv_DV_Next
         lem_ind_inv_dv_next_ind_inv_helper_2(dv, e, dv');    
     }
 
-    lemma lem_ind_inv_dv_next_ind_inv_helper_b(dv: DVState, e: DVBlockEvent, dv': DVState)       
+    lemma lem_ind_inv_dv_next_ind_inv_helper_b(dv: Block_DVState, e: DVBlockEvent, dv': Block_DVState)       
     requires DV_Block_Proposer_Spec.NextEventPreCond(dv, e)
     requires DV_Block_Proposer_Spec.NextEvent(dv, e, dv')  
     requires ind_inv(dv) 
@@ -410,7 +410,7 @@ module Ind_Inv_DV_Next
         lem_ind_inv_dv_next_ind_inv_helper_5(dv, e, dv');    
     }
 
-    lemma lem_ind_inv_dv_next_ind_inv_helper(dv: DVState, e: DVBlockEvent, dv': DVState)       
+    lemma lem_ind_inv_dv_next_ind_inv_helper(dv: Block_DVState, e: DVBlockEvent, dv': Block_DVState)       
     requires DV_Block_Proposer_Spec.NextEventPreCond(dv, e)
     requires DV_Block_Proposer_Spec.NextEvent(dv, e, dv')  
     requires ind_inv(dv) 
@@ -434,7 +434,7 @@ module Ind_Inv_DV_Next
         lem_ind_inv_dv_next_ind_inv_helper_b(dv, e, dv');                
     }
 
-    lemma lem_ind_inv_dv_next_ind_inv(dv: DVState, e: DVBlockEvent, dv': DVState)       
+    lemma lem_ind_inv_dv_next_ind_inv(dv: Block_DVState, e: DVBlockEvent, dv': Block_DVState)       
     requires DV_Block_Proposer_Spec.NextEventPreCond(dv, e)
     requires DV_Block_Proposer_Spec.NextEvent(dv, e, dv')  
     requires ind_inv(dv)    
@@ -443,7 +443,7 @@ module Ind_Inv_DV_Next
         lem_ind_inv_dv_next_ind_inv_helper(dv, e, dv');                                  
     }
 
-    lemma lem_ind_inv_dv_ind_inv_NextPreCond(dv: DVState, dv': DVState)       
+    lemma lem_ind_inv_dv_ind_inv_NextPreCond(dv: Block_DVState, dv': Block_DVState)       
     requires DV_Block_Proposer_Spec.NextPreCond(dv)
     requires DV_Block_Proposer_Spec.Next(dv, dv')  
     requires ind_inv(dv)    
@@ -459,7 +459,7 @@ module Ind_Inv_DV_Next
     } 
 
     lemma lem_NextPreCond(
-        s: DVState
+        s: Block_DVState
     )
     requires ind_inv(s)
     ensures  NextPreCond(s)                
